src/AsyncFS.v
@@ -917,19 +917,19 @@ Module AFS.
       LOG.rep (FSXPLog fsxp) (SB.rep fsxp) (LOG.NoTxn ds) (MSLL mscs) hm *
       [[[ ds!! ::: (Fm * DIRTREE.rep fsxp Ftop tree ilist frees) ]]] *
       [[ DIRTREE.find_subtree pathname tree = Some (DIRTREE.TreeDir dnum tree_elem) ]]
-    POST:hm RET:^(mscs', ok)
+    POST:hm' RET:^(mscs', ok)
       [[ MSAlloc mscs' = MSAlloc mscs ]] *
      ([[ ok = false ]] *
-        LOG.rep (FSXPLog fsxp) (SB.rep fsxp) (LOG.NoTxn ds) (MSLL mscs') hm   \/
+        LOG.rep (FSXPLog fsxp) (SB.rep fsxp) (LOG.NoTxn ds) (MSLL mscs') hm'   \/
       [[ ok = true ]] * exists d tree' ilist' frees',
-        LOG.rep (FSXPLog fsxp) (SB.rep fsxp) (LOG.NoTxn (pushd d ds)) (MSLL mscs') hm *
+        LOG.rep (FSXPLog fsxp) (SB.rep fsxp) (LOG.NoTxn (pushd d ds)) (MSLL mscs') hm' *
         [[ tree' = DIRTREE.update_subtree pathname
                       (DIRTREE.delete_from_dir name (DIRTREE.TreeDir dnum tree_elem)) tree ]] *
         [[[ d ::: (Fm * DIRTREE.rep fsxp Ftop tree' ilist' frees') ]]] *
         [[ dirtree_safe ilist  (BFILE.pick_balloc frees  (MSAlloc mscs')) tree
                         ilist' (BFILE.pick_balloc frees' (MSAlloc mscs')) tree' ]])
-    CRASH:hm
-      LOG.idempred (FSXPLog fsxp) (SB.rep fsxp) ds hm
+    CRASH:hm'
+      LOG.idempred (FSXPLog fsxp) (SB.rep fsxp) ds hm'
     >} delete fsxp dnum name mscs.
   Proof.
     unfold delete; intros.
